This proof can be curious.

HL/Equiv.lean
@@ -1,5 +1,7 @@
 import SFLMeta
 
+import LF.Typeclasses
+import HL.Imp
 
 
 open Verso.Genre Manual
@@ -11,3 +13,137 @@ tag := "Equiv"
 htmlSplit := .never
 file := some "Equiv"
 %%%
+
+
+:::dev "Sati (satiscugcat)"
+  At this point, the Rocq file provides instructions about using a new directory,
+  making sure the project is set up properly, and also instructions about how to
+  deal with the exercises. I am assuming these things are being moved to Intro.lean? 
+  I am excluding them for now.
+:::
+
+
+:::dev "Sati (satiscugcat)"
+
+```
+namespace Equiv
+
+```
+:::
+# Behavioral Equivaleence
+::::full
+
+  In an earlier chapter, we investigated the correctness of a very
+  simple program transformation: the `optimize_0plus` function.  The
+  programming language we were considering was the first version of
+  the language of arithmetic expressions -- with no variables -- so
+  in that setting it was very easy to define what it means for a
+  program transformation to be correct: it should always yield a
+  program that evaluates to the same number as the original.
+
+  To talk about the correctness of program transformations for the
+  full Imp language -- in particular, assignment -- we need to
+  consider the role of mutable state and develop a more
+  sophisticated notion of correctness, which we'll call _behavioral
+  equivalence_.
+::::
+
+::::full
+For example:
+- `X + 2` is behaviorally equivalent to `1 + X + 1`
+- `X - X` is behaviorally equivalent to `0`
+- `(X - 1) + 1` is _not_ behaviorally equivalent to `X`
+::::
+
+## Definitions
+
+::::full
+For `aexp`s and `bexp`s with variables, the definition we want is
+clear: Two `aexp`s or `bexp`s are "behaviorally equivalent" if
+they evaluate to the same result in every state.
+::::
+
+```lean
+def Aexp.equiv (a₁ a₂ : Aexp) : Prop :=
+  ∀ (st: State),
+    a₁.eval st = a₂.eval st
+```
+
+```lean
+def Bexp.equiv (b₁ b₂ : Bexp) : Prop :=
+  ∀ (st: State),
+    b₁.eval st = b₂.eval st
+```
+
+-- ::::full 
+-- Here are some simple examples of equivalences of arithmetic
+-- and boolean expressions.
+-- ::::
+
+```lean
+example : Aexp.equiv 
+          (aexp { X - X }) 
+          (aexp { 0 }) :=
+  by
+    intros st
+    simp
+```
+
+
+```lean
+example : Bexp.equiv 
+          (bexp { X - X = 0 }) 
+          (bexp { true }) :=
+  by
+    intros st
+    simp
+```
+
+::::full
+  For commands, the situation is a little more subtle.  We
+  can't simply say "two commands are behaviorally equivalent if they
+  evaluate to the same ending state whenever they are started in the
+  same initial state," because some commands, when run in some
+  starting states, don't terminate in any final state at all!
+
+  What we need instead is this: two commands are behaviorally
+  equivalent if, for any given starting state, they either (1) both
+  diverge or else (2) both terminate in the same final state.  A
+  compact way to express this is "if the first one terminates in a
+  particular state then so does the second, and vice versa."
+::::
+
+```lean
+def Com.equiv (c₁ c₂: Com) : Prop :=
+    ∀ (st st': State),
+      (st =[ c₁ ]=> st') ↔ (st =[ c₂ ]=> st')
+```
+
+## Simple Examples
+
+::::full
+  For examples of command equivalence, let's start by looking at
+  a trivial equivalence involving `skip`.
+::::
+
+```lean
+theorem skip_left: ∀ c,
+  Com.equiv
+    (imp {skip; ~c})
+    c := 
+  by
+  workinclass!
+    intros c st st'
+    constructor <;> intro h
+    case mp => 
+      cases h with
+      | seq _ _ _ _ _ h1 h2 => 
+        cases h1 with
+        | skip => assumption
+    case mpr =>
+      apply Com.EvalR.seq _ _ _ st
+      · apply Com.EvalR.skip
+      · assumption
+```
+
+
